hol/polymorphise_p4Script.py
@@ -6,20 +6,28 @@ import os
 
 filename = os.path.dirname(os.path.realpath(__file__)) + os.sep + "p4Script.sml"
 
-#Hacky, fragile rewrites
+#Ott-generated type abbreviations and Hol_datatypes that contain polymorphic types
 #TODO Perform a check that these lines are unchanged in the p4Script.sml file?
-od_hacks = OrderedDict([("val _ = type_abbrev(\"ascope\", ``:('a)``);", ""),
+od_hacks = OrderedDict([("val _ = type_abbrev(\"ascope\", ``:('a)``);", ""), #Delete this type abbreviation
                         ("val _ = Hol_datatype ` \nffblock =  (* fixed-function block *)\n   ffblock_ff of ff\n`;",
                          "val _ = Hol_datatype ` \nffblock =  (* fixed-function block *)\n   ffblock_ff of 'a ff\n`;"),
                         ("val _ = type_abbrev(\"ffblock_map\", ``:(string |-> ffblock)``);",
                          "val _ = type_abbrev(\"ffblock_map\", ``:(string |-> 'a ffblock)``);"),
                         ("val _ = type_abbrev(\"actx\", ``:(ab_list # pblock_map # ffblock_map # input_f # output_f # copyin_pbl # copyout_pbl # ext_map # func_map)``);",
                          "val _ = type_abbrev(\"actx\", ``:(ab_list # pblock_map # 'a ffblock_map # 'a input_f # 'a output_f # 'a copyin_pbl # 'a copyout_pbl # ext_map # func_map)``);"),
-                        ("val _ = type_abbrev(\"astate\", ``:(aenv # g_scope_list # arch_frame_list # ctrl # status)``);",
-                         "val _ = type_abbrev(\"astate\", ``:('a aenv # g_scope_list # arch_frame_list # ctrl # status)``);")])
+                        ("val _ = type_abbrev(\"astate\", ``:(aenv # g_scope_list # arch_frame_list # status)``);",
+                         "val _ = type_abbrev(\"astate\", ``:('a aenv # g_scope_list # arch_frame_list # status)``);"),
+                        ("val _ = type_abbrev(\"ext_fun_map\", ``:(string |-> (stmt # (string # d) list # ext_fun))``);",
+                         "val _ = type_abbrev(\"ext_fun_map\", ``:(string |-> (stmt # (string # d) list # 'a ext_fun))``);"),
+                        ("val _ = type_abbrev(\"ext_map\", ``:(string |-> (((stmt # (string # d) list # ext_fun) option) # ext_fun_map))``);",
+                         "val _ = type_abbrev(\"ext_map\", ``:(string |-> (((stmt # (string # d) list # 'a ext_fun) option) # 'a ext_fun_map))``);"),
+                        ("val _ = type_abbrev(\"ctx\", ``:(apply_table_f # ext_map # func_map # b_func_map # pars_map # tbl_map)``);",
+                         "val _ = type_abbrev(\"ctx\", ``:('a apply_table_f # 'a ext_map # func_map # b_func_map # pars_map # tbl_map)``);"),
+                        ("val _ = type_abbrev(\"actx\", ``:(ab_list # pblock_map # ffblock_map # input_f # output_f # copyin_pbl # copyout_pbl # apply_table_f # ext_map # func_map)``);",
+                         "val _ = type_abbrev(\"actx\", ``:(ab_list # pblock_map # 'a ffblock_map # 'a input_f # 'a output_f # 'a copyin_pbl # 'a copyout_pbl # 'a apply_table_f # 'a ext_map # func_map)``);")])
 
-#Straightforward, modular rewrites
-od = OrderedDict([("ascope_ty", "'a"),
+#Assign the polymorphic types (found in semantics definitions, et.c.) a proper 'a
+od = OrderedDict([("ascope_ty", "'a"), #Replace this as it appears in type abbreviations
                   (":ascope", ":'a"),
                   (":astate", ":'a astate"),
                   (":ffblock_map", ":'a ffblock_map"), 
@@ -27,7 +35,11 @@ od = OrderedDict([("ascope_ty", "'a"),
                   (":output_f", ":'a output_f"),
                   (":copyin_pbl", ":'a copyin_pbl"),
                   (":copyout_pbl", ":'a copyout_pbl"),
-                  (":ff", ":'a ff")])
+                  (":ff", ":'a ff"),
+                  (":ctx", ":'a ctx"),
+                  (":ext_map", ":'a ext_map"),
+                  (":ext_fun", ":'a ext_fun"),
+                  (":apply_table_f", ":'a apply_table_f")])
                   
 all_replaces = OrderedDict(list(od_hacks.items()) + list(od.items()))
 
@@ -39,12 +51,12 @@ def replace_all(text, dic):
 fin = open(filename, "rt")
 data = fin.read()
 
-#replace all occurrences of the required string
+#Replace all occurrences of the required string
 data = replace_all(data, all_replaces)
 
 fin.close()
 
-#output the result
+#Output the result
 fout = open(filename, "wt")
 fout.write(data)
 fout.close()
