Makefile
@@ -1,6 +1,6 @@
 default: docs/semantics/main.pdf
 
-hol/p4Script.sml: ott/p4.ott
+hol/p4Script.sml: ott/p4.ott ott/p4_sem.ott ott/p4_types.ott
 	cd hol && ott -i ../ott/p4.ott -i ../ott/p4_sem.ott -i ../ott/p4_types.ott -o p4Script.sml && python ./polymorphise_p4Script.py
 
 hol: hol/p4Script.sml hol/ottScript.sml hol/ottLib.sig hol/ottLib.sml
